Change values to set of dirty objects

simple_tm.scala
@@ -5,7 +5,6 @@
 
 type Process = BigInt
 type MemoryObject = BigInt
-type MemoryObjectValue = BigInt
 type TimeStamp = BigInt
 
 sealed abstract class Operation(obj: MemoryObject) {
@@ -21,7 +20,7 @@ case class ProcessState(
     currentOp: BigInt,
     currentSubOp: BigInt,
     readSet: Map[MemoryObject, TimeStamp],
-    writeSet: Map[MemoryObject, MemoryObjectValue]
+    writeSet: Set[MemoryObject]
 ) {
     def nextSubOp(): ProcessState =
         ProcessState(currentTx, currentOp, currentSubOp + 1, readSet, writeSet)
@@ -30,54 +29,53 @@ case class ProcessState(
         ProcessState(currentTx, currentOp + 1, 0, readSet, writeSet)
         
     def nextTx(): ProcessState =
-        ProcessState(currentTx + 1, 0, 0, Map(), Map())
+        ProcessState(currentTx + 1, 0, 0, Map(), Set())
 
     def abortTx(): ProcessState =
         ProcessState(currentTx, -1, 0, readSet, writeSet)
 
     def restartTx(): ProcessState =
-        ProcessState(currentTx, 0, 0, Map(), Map())
+        ProcessState(currentTx, 0, 0, Map(), Set())
 
     def addToReadSet(obj: MemoryObject, ts: TimeStamp): ProcessState =
         ProcessState(currentTx, currentOp, currentSubOp, readSet + (obj -> ts), writeSet)
 
-    def addToWriteSet(obj: MemoryObject, v: MemoryObjectValue): ProcessState =
-        ProcessState(currentTx, currentOp, currentSubOp, readSet, writeSet + (obj -> v))
+    def addToWriteSet(obj: MemoryObject): ProcessState =
+        ProcessState(currentTx, currentOp, currentSubOp, readSet, writeSet + obj)
 }
 
-val startProcess = ProcessState(0, 0, 0, Map(), Map())
+val startProcess = ProcessState(0, 0, 0, Map(), Set())
 
 case class SystemState(
     txQueues: Map[Process, Seq[Transaction]],
     procStates: Map[Process, ProcessState],
-    objValues: Map[MemoryObject, MemoryObjectValue],
+    dirtyObjs: Set[MemoryObject],
     lockedObjs: Set[MemoryObject],
     objTimeStamps: Map[MemoryObject, TimeStamp]
 ) {
-    def updateState(p: Process, s: ProcessState): SystemState =
-        SystemState(txQueues, procStates + (p -> s), objValues, lockedObjs, objTimeStamps)
+    def updateState(proc: Process, state: ProcessState): SystemState =
+        SystemState(txQueues, procStates + (proc -> state), dirtyObjs, lockedObjs, objTimeStamps)
     
-    def updateValue(o: MemoryObject, v: MemoryObjectValue): SystemState =
-        SystemState(txQueues, procStates, objValues + (o -> v), lockedObjs, objTimeStamps)
+    def markDirty(obj: MemoryObject): SystemState =
+        SystemState(txQueues, procStates, dirtyObjs + obj, lockedObjs, objTimeStamps)
 
-    def restoreValues(writeSet: Map[MemoryObject, MemoryObjectValue]): SystemState =
-        SystemState(txQueues, procStates, objValues ++ writeSet, lockedObjs, objTimeStamps)
+    def cleanObjects(writeSet: Set[MemoryObject]): SystemState =
+        SystemState(txQueues, procStates, dirtyObjs -- writeSet, lockedObjs, objTimeStamps)
 
-    def acquireLock(o: MemoryObject): SystemState =
-        SystemState(txQueues, procStates, objValues, lockedObjs + o, objTimeStamps)
+    def acquireLock(obj: MemoryObject): SystemState =
+        SystemState(txQueues, procStates, dirtyObjs, lockedObjs + obj, objTimeStamps)
     
-    def releaseLocks(objs: Set[MemoryObject]): SystemState =
-        SystemState(txQueues, procStates, objValues, lockedObjs -- objs, objTimeStamps)
+    def releaseLocks(writeSet: Set[MemoryObject]): SystemState =
+        SystemState(txQueues, procStates, dirtyObjs, lockedObjs -- writeSet, objTimeStamps)
     
-    def updateTimestamps(objs: Set[MemoryObject]): SystemState =
-        SystemState(txQueues, procStates, objValues, lockedObjs,
-            objTimeStamps.map{case (o,ts) =>  if(objs.contains(o)) (o, ts + 1) else (o, ts)})
+    def updateTimestamps(writeSet: Set[MemoryObject]): SystemState =
+        SystemState(txQueues, procStates, dirtyObjs, lockedObjs,
+            objTimeStamps.map{case (o,ts) =>  if(writeSet.contains(o)) (o, ts + 1) else (o, ts)})
 }
 
 def startSystem(txQueues: Map[Process, Seq[Transaction]]): SystemState = {
     var procStates = txQueues.mapValues(_ => startProcess)
     var objs = txQueues.values.flatten.flatten(tx => tx.ops).map(op => op.o).toSet
-    var objValues = objs.map(o => (o, BigInt(0))).toMap
     var objTimeStamps = objs.map(o => (o, BigInt(0))).toMap
-    SystemState(txQueues, procStates, objValues, Set(), objTimeStamps)
+    SystemState(txQueues, procStates, Set(), Set(), objTimeStamps)
 }
